First small-step formalized (inactive to active process), by carrying a proof that the local scheduler always gives back a callsite of the appropriate class

src/semantics.lean
@@ -2,6 +2,8 @@
 
 import syntax data.finsupp
 
+universe u
+
 open signature type pexp nat list
 
 /- Fix a signature (and global names). We treat object identities transparently. Each object identity is associated to a single class name. Given a finite set of object identities, there can always be a fresh object identity not in that set (thanks to Johannes Hölzl). Allocation of a fresh object results in an object with the same class name as allocated. Equality is decidable for objects. -/
@@ -23,89 +25,117 @@ instance objects.decidable : decidable_eq β :=
 
 /- We treat values as being of a type. A value of a reference type is an object of the same class, or null. A value of a data type is a term of the type in the host language. -/
 @[derive decidable_eq]
-inductive value (β : Type) [objects α β] : type α → Type 1
+inductive value [objects α β] : type α → Type 1
 | object {c : class_name α} (o : β)
     (H : c = class_of α o) : value (ref c)
 | null (c : class_name α) : value (ref c)
 | term {γ : datatype} : γ → value (data α γ)
-instance value.inhabited : Π{ty : type α}, inhabited (value β ty)
+instance value.inhabited [objects α β] :
+    Π{ty : type α}, inhabited (value ty)
 | (ref c) := ⟨value.null c⟩
-| (data .(α) γ) := ⟨value.term β γ.default⟩
+| (data .(α) γ) := ⟨value.term γ.default⟩
 -- Projection of value to term
-def value.unterm {γ : datatype} :
-    Π (x : value β (data α γ)), γ.host
-| (value.term .(β) t) := t
+def value.unterm [objects α β] {γ : datatype} :
+    Π (x : value (data α γ)), γ.host
+| (value.term t) := t
 -- Projection of value to object
 def value.unobject {c : class_name α} :
-    Π (x : value β (ref c)), option β
+    Π (x : value (ref c)), option β
 | (value.object o _) := o
 | (value.null _) := none
+def value.not_null [objects α β] {c : class_name α} (x : value (ref c)) : Prop := x ≠ value.null c
+-- Projection of value to object (guarantee)
+def value.the_object {c : class_name α} :
+    Π (x : value (ref c)), value.not_null x → β
+| (value.object o _) _ := o
+| (value.null .(c)) G := begin exfalso, apply G, refl end
+lemma value.class_of_the_object [objects α β] {c : class_name α}
+  {x : value (ref c)} (G : value.not_null x) :
+  class_of α (value.the_object x G) = c :=
+begin
+  cases x,
+  {unfold value.the_object, apply eq.symm, assumption},
+  {exfalso, apply G, refl}
+end
 
-/- For class C we have a state space Σ(C) consisting of an assignment of fields to values. For method m, we have a argument space Σ(m) consisting of an assignment of method parameters to values. Given a list of types, we have a value list of values with matching types. An object space consists of: a this identity, a state space (of the self class). -/
+/- For class C we have a state space Σ(C) consisting of a this identity and an assignment of fields to values. For method m, we have a argument space Σ(m) consisting of an assignment of method parameters to values. -/
 @[derive decidable_eq]
-structure arg_space (β : Type) [objects α β]
+structure arg_space [objects α β]
     {self : class_name α} (m : method_name self) :=
-  (map (p : param_name m) : value β (param_type p))
-structure state_space (β : Type) [objects α β]
-    (self : class_name α) :=
-  (map (f : field_name self) : value β (field_type f))
-inductive vallist (β : Type) [objects α β] :
-    list (type α) → Type 1
+  (map (p : param_name m) : value (param_type p))
+structure state_space [objects α β] (self : class_name α) :=
+  (map (f : field_name self) : value (field_type f))
+  (this : value (ref self))
+  (H : value.not_null this)
+def state_space.id [objects α β] {self : class_name α}
+  (σ : state_space self) : β := value.the_object σ.this σ.H
+lemma state_space.class_of_id [objects α β] {self : class_name α}
+  (σ : state_space self) : class_of α σ.id = self :=
+begin
+  unfold state_space.id, apply value.class_of_the_object
+end
+notation Σ(m) := arg_space m
+notation Σ(C) := state_space C
+
+/- Given a list of types, we have a value list of values with matching types. -/
+inductive vallist [objects α β] : list (type α) → Type 1
 | nil : vallist []
 | cons {ty : type α} {l : list (type α)} :
-  value β ty → vallist l → vallist (ty::l)
-def vallist.default (β : Type) [objects α β] :
-    Π(l : list (type α)), vallist β l
-| [] := vallist.nil β
-| (t :: l) := vallist.cons (default (value β t))
+  value ty → vallist l → vallist (ty::l)
+def vallist.default [objects α β] :
+    Π(l : list (type α)), vallist l
+| [] := vallist.nil
+| (t :: l) := vallist.cons (default (value t))
     (vallist.default l)
-instance vallist.inhabited (l : list (type α)) :
-  inhabited (vallist β l) := ⟨vallist.default β l⟩
-structure object_space (β : Type) [objects α β]
-    (self : class_name α) :=
-  (val : value β (ref self))
-  (state : state_space β self)
-
-variables {self : class_name α}
-
-/- An active process consists of: an argument space (of the current method), a value list (of the local variables), and a statement. -/
-structure active_process (this : object_space β self)
-    (e : tenv self) :=
-  (args : arg_space β e.current) (store : vallist β e.locals)
-  (stmt : stmt e)
+instance vallist.inhabited [objects α β] (l : list (type α)) :
+  inhabited (vallist l) := ⟨vallist.default l⟩
 /- Given a value list and an index in the list of types, we obtain a value. -/
-def vallist.lookup : Π {l : context α} {ty : type α},
-    vallist β l → list_at ty l → value β ty
-| (x :: xs) ._ (vallist.cons (v : value β x) _)
+def vallist.lookup [objects α β] {ty : type α} :
+    Π {l : context α}, vallist l → list_at ty l → value ty
+| (x :: xs) (vallist.cons (v : value x) _)
   (list_at.here .(x) .(xs)) := v
-| (x :: xs) ty (vallist.cons _ (ys : vallist β xs))
+| (x :: xs) (vallist.cons _ (ys : vallist xs))
   (list_at.tail .(x) (zs : list_at .(ty) xs)) :=
     vallist.lookup ys zs
--- Given an active process, we can lookup the value of a read variable.
-variables {this : object_space β self} {e : tenv self}
-def active_process.lookup (P : active_process this e)
-    {tx : type α} : rvar e tx → value β tx
-| (rvar.tvar t) := eq.mpr (congr_arg _ t.H) this.val
-| (rvar.fvar f) := eq.mpr (congr_arg _ f.H) $ this.state.map f.idx
-| (rvar.pvar p) := eq.mpr (congr_arg _ p.H) $ P.args.map p.idx
-| (rvar.lvar l) := P.store.lookup l.idx
-/- Evaluating a pure expression in an active process. -/
-def eval (P : active_process this e) : Π {ty : type α},
-    pexp e ty → value β ty
-| bool (requal l r) := value.term β $ to_bool (eval l = eval r)
-| _ (lookup r) := P.lookup r
-| _ (const _ v) := value.term β v
-| _ (apply f r) := value.term β $ f (eval r).unterm
+
+variables {C : class_name α} {e : tenv C}
+
+/- An active process consists of: an argument space (of the current method), a value list (of the local variables), and a list of statements. -/
+structure active_process (e : tenv C) :=
+  (args : Σ(e.current)) (store : vallist e.locals)
+  (body : list (statement e))
+/- Given an object space and active process, we can lookup the value of a read variable. -/
+def active_process.lookup (π : active_process e) (σ : Σ(C))
+    {tx : type α} : rvar e tx → value tx
+| (rvar.tvar t) := eq.mpr (congr_arg _ t.H) $ σ.this
+| (rvar.fvar f) := eq.mpr (congr_arg _ f.H) $ σ.map f.idx
+| (rvar.pvar p) := eq.mpr (congr_arg _ p.H) $ π.args.map p.idx
+| (rvar.lvar l) := π.store.lookup l.idx
+/- Evaluating a pure expression, Val(p)(σ,π). -/
+def eval (σ : Σ(C)) (π : active_process e) :
+    Π {ty : type α}, pexp e ty → value ty
+| bool (requal l r) := value.term $ to_bool (eval l = eval r)
+| _ (lookup r) := π.lookup σ r
+| _ (const _ v) := value.term v
+| _ (apply f r) := value.term $ f (eval r).unterm
 /- A process is either nil or an active process. -/
-inductive process (this : object_space β self)
+inductive process {α : Type} [objects α β] (C : class_name α)
 | nil : process
-| active {e : tenv self} (a : active_process this e) : process
+| active (e : tenv C) (a : active_process e) : process
+
 /- An event is either an asynchronous method call of some caller object to a callee object, its method, and for each parameter an argument value. Or, an event is a method selection. -/
 @[derive decidable_eq]
 structure callsite (α β : Type) [objects α β] :=
   (o : β)
   (m : method_name (class_of α o))
-  (τ : arg_space β m)
+  (τ : Σ(m))
+def callsite.elim {γ : Sort u} (c : callsite α β)
+    (f : Π(o : β) (m : method_name (class_of α o)) (τ : Σ(m)),
+      c = ⟨o,m,τ⟩ → γ) : γ :=
+  match c, rfl : (∀ b, c = b → γ) with
+  | ⟨o,m,τ⟩, h := f o m τ h
+  end
+
 @[derive decidable_eq]
 inductive event (α β : Type) [objects α β]
 | call: β → callsite α β → event
@@ -115,28 +145,125 @@ def event.to_callsite : event α β → callsite α β
 | (event.selection c) := c
 instance event.event_to_callsite : has_coe (event α β)
   (callsite α β) := ⟨event.to_callsite⟩
+
 /- A global history is a sequence of events. -/
 @[reducible]
 def global_history (α β : Type) [objects α β] := list (event α β)
 /- There are two subsequences of a global history. The first consists only of call events with the object as callee (abstracted to its corresponding call site), the second consists only of selection events with the object as callee. -/
-def event.is_call_to (α : Type) [objects α β] (x : β) :
+def event.is_call_to {α : Type} [objects α β] (x : β) :
     event α β → option (callsite α β)
 | (event.call _ c) := if x = c.o then some c else none
 | _ := none
-def event.is_selection_of (α : Type) [objects α β] (x : β) :
+/- Call events to an object are of that object. -/
+@[simp]
+lemma event.is_call_to_object {x : β} {e : event α β}
+  {c : callsite α β} : event.is_call_to x e = some c →
+  c.o = x :=
+begin
+  intro, cases e; simp [event.is_call_to] at a,
+  { by_cases (x = e_a_1.o); simp [h] at a,
+    rewrite h, rewrite ← a, exfalso, assumption },
+  { exfalso, assumption }
+end
+def event.is_selection_of {α : Type} [objects α β] (x : β) :
     event α β → option (callsite α β)
 | (event.selection c) := if x = c.o then some c else none
 | _ := none
+/- Selection events of an object are of that object. -/
+@[simp]
+lemma event.is_selection_of_object {x : β} {e : event α β}
+  {c : callsite α β} : event.is_selection_of x e = some c →
+  c.o = x :=
+begin
+  intro, cases e; simp [event.is_selection_of] at a,
+  { exfalso, assumption },
+  { by_cases (x = e.o); simp [h] at a,
+    rewrite h, rewrite ← a, exfalso, assumption }
+end
+/- The subsequences are obtained by filtering out events. -/
 def global_history.calls_to (θ : global_history α β)
     (x : β) : list (callsite α β) :=
-  θ.filter_map (event.is_call_to α x)
+  θ.filter_map (event.is_call_to x)
 def global_history.selections_of (θ : global_history α β)
     (x : β) : list (callsite α β) :=
-  θ.filter_map (event.is_selection_of α x)
+  θ.filter_map (event.is_selection_of x)
 reserve notation `!`:68
 reserve notation `?`:68
 infix ! := global_history.calls_to
 infix ? := global_history.selections_of
+/- The list of pending calls to an object is the list of calls to, with the selections removed. -/
+def global_history.pending_calls_to (θ : global_history α β)
+  (o : β) : list (callsite α β) := (θ!o).remove_all (θ?o)
+/- Pending calls have the same object as requested. -/
+lemma global_history.pending_calls_to_object
+  (θ : global_history α β) (o : β) :
+  ∀ c : callsite α β,
+    c ∈ (global_history.pending_calls_to θ o) → c.o = o :=
+begin
+  unfold global_history.pending_calls_to, intro,
+  suffices : c ∈ θ!o → c.o = o, intro, apply this,
+  simp [remove_all] at a, cases a, assumption,
+  simp [global_history.calls_to], intro, intro,
+  apply event.is_call_to_object
+end
+/- We have an optional first pending call to an object. -/
+def global_history.sched (θ : global_history α β)
+    (o : β) : option (callsite α β) :=
+  head (lift (θ.pending_calls_to o))
+/- Scheduled calls have the same object as requested. -/
+lemma global_history.sched_object (θ : global_history α β)
+  (o : β) (c : callsite α β) :
+  (global_history.sched θ o) = some c → c.o = o :=
+begin
+  unfold global_history.sched,
+  cases H : (global_history.pending_calls_to θ o),
+  { intro, exfalso, apply head_lift_nil a },
+  { intro, have : hd = c, apply tail_lift_some a,
+    apply global_history.pending_calls_to_object θ,
+    rewrite H, rewrite this, simp }
+end
+
+/- We fix a program, and global history. -/
+variables (p : program α) (θ : global_history α β)
+/- A local configuration is an object identity and a process. -/
+structure local_config (β : Type) [objects α β]
+  (C : class_name α) := (σ : Σ(C)) (m : process C)
+/- Given a method and arguments, we can activate a process. -/
+def process.activate (C : class_name α) (m : method_name C)
+    (τ : Σ(m)) : process C :=
+  process.active (p.body m).tenv ⟨τ,default _,(p.body m).S⟩
+
+/- A step is taken on a local configuration. -/
+def local_config.step : local_config β C → option ((local_config β C) × option (event α β))
+    
+/- If the process is inactive, we obtain a pending method call. If no method call is pending, no step is taken. Otherwise, the next local configuration is an active process with the arguments of the selected method, a default store, and the body of the method as statement; additionally, a selection event is generated. -/
+| ⟨σ, process.nil .(C)⟩ := let c := θ.sched σ.id in
+    option.elim c (λh, none) (λd h, callsite.elim d (λo m τ g,
+      let p := process.activate p (class_of α o) m τ,
+        H : class_of α o = C := begin
+          have : (θ.sched σ.id) = some ⟨o, m, τ⟩,
+            rw ← g, assumption,
+          have : state_space.id σ = o,
+            apply eq.symm,
+            apply global_history.sched_object θ (σ.id) ⟨o,m,τ⟩,
+            assumption,
+          rewrite ← this,
+          apply state_space.class_of_id
+        end
+      in some ⟨⟨σ, cast (congr_arg _ H) p⟩, event.selection d⟩))
+/- Otherwise, there is an active process. We look at the list of statements. If the list is empty, the process becomes inactive. -/
+/- Otherwise, there is a current statement. If the current statement is an if statement, for which we evaluate the boolean pure expression. If it is true, we replace the current statement by those of the then-branch. Otherwise, we replace the current statement by those of the else-branch. -/
+/- Otherwise, there is a while statement. We evaluate the boolean pure expression. If it is true, we prepend the body to the current statements. Otherwise, we discard the current statement. -/
+/- Otherwise, we consider the assignment statement. We evaluate the pure expression, and the result is taken to update the variable on the left-hand side: if it is a field then the object space field state is updated, otherwise it is a local and the store is updated. In both cases, the current statement is discarded. -/
+/- Otherwise, we have an async statement. We evaluate the argument list to a value list; the object pure expression is evaluated to an object value. If that value is null, no step is taken. Otherwise, we generate a method selection event with our object as caller and the appropriate call site, and discard the current statement. -/
+/- Otherwise, we have an alloc statement. We evaluate the argument list to a value list. A fresh object identity is obtained from the global history. A method selection event to the constructor of the freshly obtained object is generated with an approriate call site, and the current statement is discarded. -/
+
+/- A global configuration is a finite set of object configurations and a global history. -/
+structure global_config (α β : Type) [objects α β] :=
+  (Γ (self : class_name α): finset (local_config β self))
+  (θ: global_history α β)
+
+-- TODO: move to some other place
 /- A local history is obtained from a global history and an object identity: it consists of the outgoing calls, an method selections involving the object. -/
 @[reducible]
 def event.is_local_to (α : Type) [objects α β] (x : β) :
@@ -146,36 +273,5 @@ def event.is_local_to (α : Type) [objects α β] (x : β) :
 instance event.decidable_local (o : β) (e: event α β) :
     decidable (event.is_local_to α o e) :=
   begin cases e; apply_instance end
-def local_history (θ : global_history α β) (o : β) :=
-  θ.filter (event.is_local_to α o)
-/- The list of pending calls to an object is the list of calls to, with the selections removed. -/
-def global_history.pending_calls_to (θ : global_history α β)
-  (o : β) : list (callsite α β) := (θ!o).remove_all (θ?o)
-/- We have an optional first pending call to an object. -/
-def global_history.sched (θ : global_history α β)
-    (o : β) : option (callsite α β) :=
-  head (lift (θ.pending_calls_to o))
-
-/- A local configuration is an object identity and a process. -/
-structure local_config (β : Type) [objects α β]
-    (self : class_name α) :=
-  (σ : object_space β self)
-  (m : process σ)
-/- We fix a program, and global history. -/
-variables (p : program α) (θ : global_history α β)
-/- A step is taken on a local configuration. -/
-def local_config.step : local_config β self →
-    option ((local_config β self) × option (event α β)) :=
-/- If the process is inactive, we obtain a pending method call. If no method call is pending, no step is taken. Otherwise, the next local configuration is an active process with the arguments of the selected method, a default store, and the body of the method as statement; additionally, an event is generated. -/
-/- Otherwise, there is an active process. We look at the list of statements. If the list is empty, the process becomes inactive. -/
-/- Otherwise, there is a current statement. If the current statement is an if statement, for which we evaluate the boolean pure expression. If it is true, we replace the current statement by those of the then-branch. Otherwise, we replace the current statement by those of the else-branch. -/
-/- Otherwise, there is a while statement. We evaluate the boolean pure expression. If it is true, we prepend the body to the current statements. Otherwise, we discard the current statement. -/
-/- Otherwise, we consider the assignment statement. We evaluate the pure expression, and the result is taken to update the variable on the left-hand side: if it is a field then the object space field state is updated, otherwise it is a local and the store is updated. In both cases, the current statement is discarded. -/
-/- Otherwise, we have an async statement. We evaluate the argument list to a value list; the object pure expression is evaluated to an object value. If that value is null, no step is taken. Otherwise, we generate a method selection event with our object as caller and the appropriate call site, and discard the current statement. -/
-/- Otherwise, we have an alloc statement. We evaluate the argument list to a value list. A fresh object identity is obtained from the global history. A method selection event to the constructor of the freshly obtained object is generated with an approriate call site, and the current statement is discarded. -/
-  sorry
-
-/- A global configuration is a finite set of object configurations and a global history. -/
-structure global_config (α β : Type) [objects α β] :=
-  (Γ (self : class_name α): finset (local_config β self))
-  (θ: global_history α β)
+def local_history (θ : global_history α β) (x : β) :=
+  θ.filter (event.is_local_to α x)
